% Copyright (c)  2025  anonymoose0.
%    Permission is granted to copy, distribute and/or modify this document
%    under the terms of the GNU Free Documentation License, Version 1.3
%    or any later version published by the Free Software Foundation;
%    with no Invariant Sections, no Front-Cover Texts, and no Back-Cover Texts.
%    A copy of the license is included in the section entitled "GNU
%    Free Documentation License".

\begin{minipage}{\textwidth}
    \textbf{Definition of the Imaginary Unit:}
    \\ \( i^2 = -1 \)
\end{minipage}

\subsection*{Formulae}
\begin{minipage}{\textwidth}
    \textbf{Distance Formula:}
    \\ \( D = \sqrt{ x^2 + y^2 } \)
\end{minipage}
\\ \begin{minipage}{\textwidth}
    \textbf{Slope Formula:}
    \\ \( m = \displaystyle\frac{ \Delta x }{ \Delta y } = \displaystyle\frac{ x_2 - x_1 }{ y_2 - y_1 } \)
\end{minipage}
\\ \begin{minipage}{\textwidth}
    \textbf{Discriminant of a Quadratic Equation:}
    \\ \( \Delta = b^2 - 4ac \)
\end{minipage}
\\ \begin{minipage}{\textwidth}
    \textbf{Quadratic Formula:}
    \\ \( x = \displaystyle\frac{ -b \pm \sqrt{ b^2 - 4ac } }{ 2a } \)
\end{minipage}
\\ \begin{minipage}{\textwidth}
    \textbf{Cubic Formula:}
    \\ \( \xi = \displaystyle\frac{ -1 + \sqrt{ -3 } }{ 2 } \)
    \\ \( \Delta_0 = b^2 - 3ac  \)
    \\ \( \Delta_1 = 2b^2 - 9abc + 27 a^2 d \)
    \\ \( C = \sqrt[3]{ \displaystyle\frac{ \Delta_1 \pm \sqrt{ \Delta_1^2 } -4 \Delta_0^3 }{ 2 } } \)
    \\ \( x_k = \displaystyle\frac{ -1 }{ 3a } \left(  b + \zeta^kC + \displaystyle\frac{ \Delta_0 }{ \zeta^k C } \right) ; k \in \{ 0, 1, 2 \} \)
\end{minipage}
\\ \begin{minipage}{\textwidth}
    \textbf{Binomial Formula:}
    \\ \( ( a + b )^n = \displaystyle\sum_{k = 0}^{n} { \binom{n}{k} a^{n - k} b^k } \)
\end{minipage}

\subsection*{Functions}
\begin{minipage}{\textwidth}
    \textbf{Slope-Intercept Form of a Line:}
    \\ \( y = mx + b \)
\end{minipage}
\\ \begin{minipage}{\textwidth}
    \textbf{Point-Slope Form of a Line:}
    \\ \( y - y_1 = m( x - x_1 ) \)
\end{minipage}
\\ \begin{minipage}{\textwidth}
    \textbf{Standard Form of a Line:}
    \\ \( Ax + By = C \)
\end{minipage}
\\ \begin{minipage}{\textwidth}
    \textbf{Exponential Function:}
    \\ \( y = a \cdot b^x \)
\end{minipage}
\\ \begin{minipage}{\textwidth}
    \textbf{Vertex Form of a Quadratic:}
    \\ \( y=  a( x - h )^2 + k \)
\end{minipage}
\\ \begin{minipage}{\textwidth}
    \textbf{Factored Form of a Quadratic:}
    \\ \( y = ( x - r_1 ) ( x - r_2 ) \)
\end{minipage}
\\ \begin{minipage}{\textwidth}
    \textbf{Standard Form of a Quadratic:}
    \\ \( y = ax^2 +bx + c \)
\end{minipage}
\\ \begin{minipage}{\textwidth}
    \textbf{Standard Form of a Polynomial:}
    \\ \( ax^n + bx^{n-1} + cx^{n-2}... + vx^2 + wx + z = 0 \)
\end{minipage}
\\ \begin{minipage}{\textwidth}
    \textbf{Standard Form of an Absolute Value Function:}
    \\ \( y = a| x - h | + k \)
\end{minipage}
\\ \begin{minipage}{\textwidth}
    \textbf{Standard Form of a Square Root Function:}
    \\ \( y = a \sqrt{ x - h } + k \)
\end{minipage}

\subsection*{Conic Sections}
\begin{minipage}{\textwidth}
    \textbf{Equation of a Circle:}
    \\ \( x^2 + y^2 = r^2 \)
\end{minipage}
\\ \begin{minipage}{\textwidth}
    \textbf{Equation of a Horizontal Ellipse:}
    \\ \( \displaystyle\frac{ ( x - h )^2 }{ a^2 } + \displaystyle\frac{ ( y - k )^2 }{ b^2 } = 1 \)
\end{minipage}
\\ \begin{minipage}{\textwidth}
    \textbf{Equation of a Vertical Ellipse:}
    \\ \( \displaystyle\frac{ ( x - h )^2 }{ b^2 } + \displaystyle\frac{ ( y - k )^2 }{ a^2 } = 1 \)
\end{minipage}
\\ \begin{minipage}{\textwidth}
    \textbf{Equation of a Horizontal Hyperbola:}
    \\ \( \displaystyle\frac{ ( x - h )^2 }{ a^2 } - \displaystyle\frac{ ( y - k )^2 }{ b^2 } = 1 \)
\end{minipage}
\\ \begin{minipage}{\textwidth}
    \textbf{Equation of a Vertical Hyperbola:}
    \\ \( \displaystyle\frac{ ( y - k )^2 }{ a^2 } - \displaystyle\frac{ ( x - h )^2 }{ b^2 } = 1 \)
\end{minipage}
\\ \begin{minipage}{\textwidth}
    \textbf{Equation of a Horizontal Parabola:}
    \\ \( x = \displaystyle\frac{ 1 }{ 4p } (y - k)^2 +h \)
\end{minipage}
\\ \begin{minipage}{\textwidth}
    \textbf{Equation of a Vertical Parabola:}
    \\ \( y = \displaystyle\frac{ 1 }{ 4p } (x - h)^2 +k \)
\end{minipage}
\\ \begin{minipage}{\textwidth}
    \textbf{Standard Form of a Conic Section:}
    \\ \( ax^2 + bxy + cy^2 + dx + ey + f = 0 \)
\end{minipage}

\subsection*{Sequences and Series}
\begin{minipage}{\textwidth}
    \textbf{Recursive Arithmetic Sequence:}
    \\ \( a_1 = x \)
    \\ \( a_n = a_{n - 1} + d \)
\end{minipage}
\\ \begin{minipage}{\textwidth}
    \textbf{Explicit Arithmetic Sequence:}
    \\ \( a_n = d( n - 1 ) + a_1 \)
\end{minipage}
\\ \begin{minipage}{\textwidth}
    \textbf{Recursive Geometric Sequence:}
    \\ \( a_1 = x \)
    \\ \( a_n = a_{n - 1} \cdot r \)
\end{minipage}
\\ \begin{minipage}{\textwidth}
    \textbf{Explicit Geometric Sequence:}
    \\ \( a_n = a_1 ( r )^{n - 1} \)
\end{minipage}
\\ \begin{minipage}{\textwidth}
    \textbf{Sum of an Arithmetic Series when the Last Term is Given:}
    \\ \( S_n = \displaystyle\frac{ n( a_1 + a_n ) }{ 2 } \)
\end{minipage}
\\ \begin{minipage}{\textwidth}
    \textbf{Sum of an Arithmetic Series when the Last Term is Not Given:}
    \\ \( S_n = \displaystyle\frac{ n( 2a_1 + d( n - 1 ) ) }{ 2 } \)
\end{minipage}
\\ \begin{minipage}{\textwidth}
    \textbf{Sum of a Geometric Series:}
    \\ \( S_n = \displaystyle\frac{ a_1 ( 1 - r^n ) }{ 1 - r } \)
\end{minipage}
\\ \begin{minipage}{\textwidth}
    \textbf{Sum of an Infinite Geometric Series:}
    \\ \( S = \displaystyle\frac{ a_1 }{ 1 - r } ; 0 < | x | < 1 \)
\end{minipage}

\subsection*{Methods}
\begin{minipage}{\textwidth}
    \textbf{Difference of Squares:}
    \\ \( a^2 - b^2 = ( a + b ) ( a - b ) \)
\end{minipage}
\\ \begin{minipage}{\textwidth}
    \textbf{Sum of Squares:}
    \\ \( a^2 + b^2 = ( a + bi ) ( a - bi ) \)
\end{minipage}
\\ \begin{minipage}{\textwidth}
    \textbf{Difference of Cubes:}
    \\ \( a^3 - b^3 = ( a - b )( a^2 + ab + b^2 ) \)
\end{minipage}
\\ \begin{minipage}{\textwidth}
    \textbf{Sum of Cubes:}
    \\ \( a^3 + b^3 = ( a + b )( a^2 - ab + b^2 ) \)
\end{minipage}
\\ \begin{minipage}{\textwidth}
    \textbf{Various Summation of Single Terms:}
    \\ \( \displaystyle\sum_{k = 1}^n { k } = \displaystyle\frac{ n( n + 1 ) }{ 2 } \)
    \\ \( \displaystyle\sum_{k = 1}^n { k^2 } = \displaystyle\frac{ n( n + 1 )( 2n + 1 ) }{ 6 } \)
    \\ \( \displaystyle\sum_{k = 1}^n { k^3 } = \displaystyle\frac{ n^2( n + 1 )^2 }{ 4 } \)
    \\ \( \displaystyle\sum_{k = 1}^n { k^4 } = \displaystyle\frac{ n( 2n + 1 )( n + 1 )( 3n^2 + 3n - 1 ) }{ 30 } \)
    \\ \( \displaystyle\sum_{k = 1}^n { k^5 } = \displaystyle\frac{ n^2 ( 2n^2 + 2n - 1 )( n + 1 )^2 }{ 12 } \)
    \\ \( \displaystyle\sum_{k = 1}^n { k^6 } = \displaystyle\frac{ n( 2n + 1 )( n + 1 )( 3n^4 + 6n^3 - 3n + 1 ) }{ 42 } \)
    \\ \( \displaystyle\sum_{k = 1}^n { k^7 } = \displaystyle\frac{ n^2 ( 3n^4 + 6n^3 - n^2 - 4n + 2 )( n + 1 )^2 }{ 24 } \)
\end{minipage}