% Copyright (c)  2025  anonymoose0.
%    Permission is granted to copy, distribute and/or modify this document
%    under the terms of the GNU Free Documentation License, Version 1.3
%    or any later version published by the Free Software Foundation;
%    with no Invariant Sections, no Front-Cover Texts, and no Back-Cover Texts.
%    A copy of the license is included in the section entitled "GNU
%    Free Documentation License".

\begin{minipage}{\textwidth}
    \textbf{Definition of Hyperbolic Sine:}
    \\ \( \sinh x = \displaystyle\frac{ e^x - e^{-x} }{ 2 } = -i \sin ix \)
\end{minipage}
\\ \begin{minipage}{\textwidth}
    \textbf{Definition of Hyperbolic Cosine:}
    \\ \( \cosh x = \displaystyle\frac{ e^x + e^{-x} }{ 2 } = \cos ix \)
\end{minipage}
\\ \begin{minipage}{\textwidth}
    \textbf{Definition of Hyperbolic Tangent:}
    \\ \( \tanh x = \displaystyle\frac{ e^x - e^{-x} }{ e^x + e^{-x} } = -i \tan ix \)
\end{minipage}
\\ \begin{minipage}{\textwidth}
    \textbf{Definition of Hyperbolic Cosecant:}
    \\ \( \text{csch } x = \displaystyle\frac{ 2 }{ e^x - e^{-x} } = i \csc ix \)
\end{minipage}
\\ \begin{minipage}{\textwidth}
    \textbf{Definition of Hyperbolic Secant:}
    \\ \( \text{sech } x = \displaystyle\frac{ 2 }{ e^x + e^{-x} } = \sec ix \)
\end{minipage}
\\ \begin{minipage}{\textwidth}
    \textbf{Definition of Hyperbolic Cotangent:}
    \\ \( \coth x = \displaystyle\frac{ e^x + e^{-x} }{ e^x - e^{-x} } = i \cot ix \)
\end{minipage}
\\ \begin{minipage}{\textwidth}
    \textbf{Hyperbolic Pythagorean Identities:}
    \\ \( \sinh^2 x - \cosh^2 x = 1 \)
    \\ \( 1 - \tanh^2 x = \text{sech}^2 \text{ } x \)
    \\ \( \coth^2 x - 1 = \text{csch}^2 \text{ } x \)
\end{minipage}
\\ \begin{minipage}{\textwidth}
    \textbf{Hyperbolic Sum/Difference Identities:}
    \\ \( \sinh( x \pm y ) = \sinh( x ) \cdot \cosh( y ) \pm \cosh( x ) \cdot \sinh( y ) \)
    \\ \( \cosh( x \pm y ) = \cosh( x ) \cdot \cosh( y ) \pm \sinh( x ) \sinh( y ) \)
    \\ \( \tanh( x \pm y ) = \displaystyle\frac{ \tanh( x ) \pm \tanh( y ) }{ 1 \pm \tanh( x ) \cdot \tanh( y ) } \)
\end{minipage}
\\ \begin{minipage}{\textwidth}
    \textbf{Hyperbolic Double Angle Identities:}
    \\ \( \sinh( 2x ) = 2 \sinh( x ) \cdot \cosh( x ) \)
    \\ \( \cosh( 2x ) = \sinh^2( x ) + \cosh^2( x ) \)
    \\ \( \tanh( 2x ) = \displaystyle\frac{ 2 \tanh( x ) }{ 1 + \tanh^2( x ) } \)
\end{minipage}
\\ \begin{minipage}{\textwidth}
    \textbf{Hyperbolic Half Angle Identities:}
    \\ \( \sinh \left( \displaystyle\frac{ x }{ 2 } \right) = \text{sgn}( x ) \sqrt{ \displaystyle\frac{ \cosh( x ) - 1 }{ 2 } } \)
    \\ \( \cosh \left( \displaystyle\frac{ x }{ 2 } \right) = \sqrt{ \displaystyle\frac{ \cosh( x ) + 1 }{ 2 } } \)
    \\ \( \tanh \left( \displaystyle\frac{ x }{ 2 } \right) = \displaystyle\frac{ \sinh( x ) }{ \cosh( x ) + 1 } \)
\end{minipage}
\\ \begin{minipage}{\textwidth}
    \textbf{Hyperbolic Sum to Product Identities:}
    \\ \( \sinh( x ) + \sinh( y ) = 2 \sinh \left( \displaystyle\frac{ x + y }{ 2 } \right) \cosh \left( \displaystyle\frac{ x - y }{ 2 } \right) \)
    \\ \( \sinh( x ) - \sinh( y ) = 2 \cosh \left( \displaystyle\frac{ x + y }{ 2 } \right) \sinh \left( \displaystyle\frac{ x - y }{ 2 } \right) \)
    \\ \( \cosh( x ) + \cosh( y ) = 2 \cosh \left( \displaystyle\frac{ x + y }{ 2 } \right) \cosh \left( \displaystyle\frac{ x - y }{ 2 } \right) \)
    \\ \( \cosh( x ) - \cosh( y ) = -2 \sinh \left( \displaystyle\frac{ x + y }{ 2 } \right) \sinh \left( \displaystyle\frac{ x - y }{ 2 } \right) \)
\end{minipage}