% Copyright (c)  2025  anonymoose0.
%    Permission is granted to copy, distribute and/or modify this document
%    under the terms of the GNU Free Documentation License, Version 1.3
%    or any later version published by the Free Software Foundation;
%    with no Invariant Sections, no Front-Cover Texts, and no Back-Cover Texts.
%    A copy of the license is included in the section entitled "GNU
%    Free Documentation License".

\begin{minipage}{\textwidth}
    \textbf{Definition of the Derivative:}
    \\ \( \displaystyle\frac{ d }{ dx } f( x ) = \displaystyle\lim_{h \rightarrow{0}} { \displaystyle\frac{ f( x + h ) - f( h ) }{ h } } = \displaystyle\lim_{x \rightarrow{a}} { \displaystyle\frac{ f( x ) - f( a ) }{ x - a } } \)
\end{minipage}
\\ \begin{minipage}{\textwidth}
    \textbf{Definition of the Taylor Series:}
    \\ \( f_a( x ) = \displaystyle\sum_{n = 0}^{\infty} { \displaystyle\frac{ \frac{ d }{ dx } f( a ) }{ n! } ( x - a )^n } \)
\end{minipage}
\\ \begin{minipage}{\textwidth}
    \textbf{Newton's Method:}
    \\ \( x_1 = a \)
    \\ \( x_n = \displaystyle\frac{ -f( x_{n - 1} ) }{ \frac{ d }{ dx } f( x_{n - 1} ) } + x_{n - 1} \)
\end{minipage}
\\ \begin{minipage}{\textwidth}
    \textbf{Trigonometric Derivatives:}
    \\ \( \displaystyle\frac{ d }{ dx } \sin x = \cos x \)
    \\ \( \displaystyle\frac{ d }{ dx } \cos x = - \sin x \)
    \\ \( \displaystyle\frac{ d }{ dx } \tan x = \sec^2 x \)
    \\ \( \displaystyle\frac{ d }{ dx } \csc x = - \csc x \cdot \cot x \)
    \\ \( \displaystyle\frac{ d }{ dx } \sec x = \sec x \cdot \tan x \)
    \\ \( \displaystyle\frac{ d }{ dx } \cot x = - \csc^2 x \)
\end{minipage}
\\ \begin{minipage}{\textwidth}
    \textbf{Hyperbolic Trigonometric Derivatives:}
    \\ \( \displaystyle\frac{ d }{ dx } \sinh x = \cosh x \)
    \\ \( \displaystyle\frac{ d }{ dx } \cosh x = \sinh x \)
    \\ \( \displaystyle\frac{ d }{ dx } \tanh x = \text{sech}^2 x \)
    \\ \( \displaystyle\frac{ d }{ dx } \text{csch } x = - \text{csch } x \cdot \coth x \)
    \\ \( \displaystyle\frac{ d }{ dx } \text{sech } x = - \text{sech } x \cdot \tanh x \)
    \\ \( \displaystyle\frac{ d }{ dx } \coth x = - \text{csch}^2 x \)
\end{minipage}
\\ \begin{minipage}{\textwidth}
    \textbf{Inverse Trigonometric Derivatives:}
    \\ \( \displaystyle\frac{ d }{ dx } \arcsin x = \displaystyle\frac{ 1 }{ \sqrt{ 1 - x^2 } } \)
    \\ \( \displaystyle\frac{ d }{ dx } \arccos x = \displaystyle\frac{ -1 }{ \sqrt{ 1 - x^2 } } \)
    \\ \( \displaystyle\frac{ d }{ dx } \arctan x = \displaystyle\frac{ 1 }{ x^2 + 1 } \)
    \\ \( \displaystyle\frac{ d }{ dx } \text{arccsc } x = \displaystyle\frac{ 1 }{ | x | \sqrt{ x^2 - 1 } } \)
    \\ \( \displaystyle\frac{ d }{ dx } \text{arcsec } x = \displaystyle\frac{ -1 }{ | x | \sqrt{ x^2 - 1 } } \)
    \\ \( \displaystyle\frac{ d }{ dx } \text{arccot } x = \displaystyle\frac{ -1 }{ x^2 + 1 } \)
\end{minipage}
\\ \begin{minipage}{\textwidth}
    \textbf{Inverse Hyperbolic Trigonometric Derivatives:}
    \\ \( \displaystyle\frac{ d }{ dx } \text{arsinh } x = \displaystyle\frac{ 1 }{ \sqrt{ x^2 + 1 } } \)
    \\ \( \displaystyle\frac{ d }{ dx } \text{arcosh } x = \displaystyle\frac{ 1 }{ \sqrt{ x^2 + 1 } } ; x > 1 \)
    \\ \( \displaystyle\frac{ d }{ dx } \text{arcoth } x = \displaystyle\frac{ 1 }{ 1 - x^2 } ; | x | < 1 \)
    \\ \( \displaystyle\frac{ d }{ dx } \text{arcsch } x = \displaystyle\frac{ -1 }{ | x | \sqrt{ 1 + x^2 } } ; x \neq 0 \)
    \\ \( \displaystyle\frac{ d }{ dx } \text{arsech } x = \displaystyle\frac{ -1 }{ x \sqrt{ 1 + x^2 } } ; 0 < x < 1 \)
    \\ \( \displaystyle\frac{ d }{ dx } \text{arcoth } x = \displaystyle\frac{ 1 }{ 1 - x^2 } ; | x | > 1 \)
\end{minipage}