% Copyright (c)  2025  anonymoose0.
%    Permission is granted to copy, distribute and/or modify this document
%    under the terms of the GNU Free Documentation License, Version 1.3
%    or any later version published by the Free Software Foundation;
%    with no Invariant Sections, no Front-Cover Texts, and no Back-Cover Texts.
%    A copy of the license is included in the section entitled "GNU
%    Free Documentation License".

\begin{minipage}{\textwidth}
    \textbf{Fermat’s Last Theorem:}
    \\ \( \lnot [ \forall n \in \mathbb{Z} : [ n \ge 3 ] \exists [a, b, c \in \mathbb{Z} ] : [ a^n +b^n = c^n ] ] \)
\end{minipage}
\\ \begin{minipage}{\textwidth}
    \textbf{Fermat’s Little Theorem:}
    \\ \( \forall [ a \in \mathbb{Z} ] \land [ n \in \mathbb{P} ] [ ( a^n - a ) \bmod n = 0 ] \)
\end{minipage}
\\ \begin{minipage}{\textwidth}
    \textbf{Wilson’s Theorem:}
    \\ \( [ ( ( n - 1 )! - 1 ) \bmod n = 0 ] \iff [ n \in \mathbb{P}] \)
\end{minipage}
\\ \begin{minipage}{\textwidth}
    \textbf{The Fibonacci Sequence:}
    \\ \( F_n = F_{n - 1} + F_{n - 2} ; F_0 = 0, F_1 = 1 \)
\end{minipage}
\\ \begin{minipage}{\textwidth}
    \textbf{Definition of the Golden Ratio:}
    \\ \( \phi = \displaystyle\frac{ 1 + \sqrt{ 5 } }{ 2 } = 1 + \displaystyle\frac{ 1 }{ 1 + \displaystyle\frac{ 1 }{ 1 + \displaystyle\frac{ 1 }{ 1 + \displaystyle\frac{ 1 }{ 1 + ... } } } } \)
\end{minipage}
\\ \begin{minipage}{\textwidth}
    \textbf{Pythagorean Triples:}
    \\ \( \left. \substack{ a = m^2 - n^2 \\ b = 2mn \\ c = m^2 + n^2 } \right\} ( m > n ) \land ( m, n \in \mathbb{Z} ) \)
\end{minipage}