% Copyright (c)  2025  anonymoose0.
%    Permission is granted to copy, distribute and/or modify this document
%    under the terms of the GNU Free Documentation License, Version 1.3
%    or any later version published by the Free Software Foundation;
%    with no Invariant Sections, no Front-Cover Texts, and no Back-Cover Texts.
%    A copy of the license is included in the section entitled "GNU
%    Free Documentation License".

\begin{minipage}{\textwidth}
    \textbf{Probability Laws:}
    \\ \( P( \lnot A ) = 1 - P( A ) \)
    \\ \( P( A \lor B ) = P( A ) + P( B ) - P( A \land B ) \)
    \\ \( P( A \land B ) = P( A ) \cdot P( B | A ) \)
    \\ \( P( A | B ) = \displaystyle\frac{ P( A \land B ) }{ P( B ) } \)
\end{minipage}
\\ \begin{minipage}{\textwidth}
    \textbf{Bayes's Theorem:}
    \\ \( P( A | B ) = \displaystyle\frac{ P( B | A ) \cdot P( A ) }{ P( B ) } \)
\end{minipage}