% Copyright (c)  2025  anonymoose0.
%    Permission is granted to copy, distribute and/or modify this document
%    under the terms of the GNU Free Documentation License, Version 1.3
%    or any later version published by the Free Software Foundation;
%    with no Invariant Sections, no Front-Cover Texts, and no Back-Cover Texts.
%    A copy of the license is included in the section entitled "GNU
%    Free Documentation License".

\begin{minipage}{\textwidth}
    \textbf{L'\^{o}pital's Rule:}
    \\ \( \displaystyle\lim_{x \rightarrow{c}} { \displaystyle\frac{ f( x ) }{ g( x ) } } = \displaystyle\lim_{x \rightarrow{c}} { \displaystyle\frac{ \frac{ d }{ dx } f( x ) }{ \frac{ d }{ dx } g( x ) } }  \)
    \\ \( [ | f( c) | = | g( c ) | = \infty] \lor [ | f( c) | = | g( c ) | = 0] \)
\end{minipage}
\\ \begin{minipage}{\textwidth}
    \textbf{Squeeze Theorem:}
    \\ \( \forall f( x ) : [ g( x )\le f( x ) \le h( x ) \forall x \in [ b, c ] ] \)
    \\ \( \exists [ \displaystyle\lim_{x \rightarrow{a}} { f( x ) } ] = \displaystyle\lim_{x \rightarrow{a}} { g( x ) } = \displaystyle\lim_{x \rightarrow{a}} { h( x ) } \)
    \\ \( \iff \exists [ \displaystyle\lim_{x \rightarrow{a}} { g( x ) } = \displaystyle\lim_{x \rightarrow{a}} { h( x ) } ] \land [a \in [ b, c ]] \)
\end{minipage}
\\ \begin{minipage}{\textwidth}
    \textbf{Common Limits:}
    \\ \( \displaystyle\lim_{x \rightarrow{0} } { \displaystyle\frac{ e^x - 1 }{ x } } = 1 \)
    \\ \( \displaystyle\lim_{x \rightarrow{\infty}} { \left( 1 + \displaystyle\frac{ x }{ n } \right)^n } = e^x \)
    \\ \( \displaystyle\lim_{x \rightarrow{\infty}} { \displaystyle\frac{ \ln x }{ x } } = 0 \)
\end{minipage}
\\ \begin{minipage}{\textwidth}
    \textbf{Common Trigonometric Limits:}
    \\ \( \displaystyle\lim_{x \rightarrow{0}} { \displaystyle\frac{ \sin x }{ x } } = 1 \)
    \\ \( \displaystyle\lim_{x \rightarrow{\infty}} { \displaystyle\frac{ \sin x }{ x } } = 0 \)
    \\ \( \displaystyle\lim_{x \rightarrow{0}} { \displaystyle\frac{ -1 + \cos x }{ x } } = 0 \)
    \\ \( \displaystyle\lim_{x \rightarrow{\infty}} { \displaystyle\frac{ -1 + \cos x }{ x } } = 0 \)
    \\ \( \displaystyle\lim_{x \rightarrow{\infty}} { \displaystyle\frac{ 1 + \cos x }{ x } } = 0 \)
    \\ \( \displaystyle\lim_{x \rightarrow{0}} { \displaystyle\frac{ \tan x }{ x } } = 1 \)
\end{minipage}